Port list.v to use HOAS notation, and speed it up (?!?)
As a side effect of the HOAS notation, this file now takes half the time.
Why that happens is a mystery.

theories/Dot/examples/list.v
@@ -1,36 +1,40 @@
 From stdpp Require Import strings.
 
 From D Require Import tactics.
-From D.Dot Require Import syn exampleInfra unstampedness_binding scalaLib.
+From D.Dot Require Import syn unstampedness_binding.
 From D.Dot.typing Require Import typing_unstamped typing_unstamped_derived.
+From D.Dot.examples Require Import exampleInfra scalaLib hoas.
 
-Import DBNotation.
+Import DBNotation hoasNotation.
 
-Implicit Types (L T U: ty) (v: vl) (e: tm) (d: dm) (ds: dms) (Γ : list ty).
+Implicit Types (L T U: hty) (Γ : list ty).
+ (* (v: vl) (e: tm) (d: dm) (ds: dms) . *)
 
-Definition trueTm := tskip (tproj (tv x0) "true").
-Definition falseTm := tskip (tproj (tv x0) "false").
+Definition htrueTm bool := htskip (htproj (htv bool) "true").
+Definition hfalseTm bool := htskip (htproj (htv bool) "false").
 
 (* bool : boolImplT *)
 (* Let Γ' := boolImplT :: Γ. *)
 
-Lemma trueTyp Γ Γ'' : Γ'' ++ boolImplT :: Γ u⊢ₜ trueTm.|[ren (+length Γ'')] : p0.|[ren (+length Γ'')] @; "Boolean".
+Lemma trueTyp Γ Γ'' : Γ'' ++ boolImplT :: Γ u⊢ₜ
+  hclose (htrueTm (hx (length Γ''))) : hclose (hpx (length Γ'') @; "Boolean").
 Proof.
   have ?: length Γ'' < length (Γ'' ++ boolImplT :: Γ) by rewrite app_length /=; lia.
-  rewrite /trueTm /= -(iterate_S tskip 0).
-  apply (Subs_typed (T1 := ▶ pv (ids (length Γ'')) @; "Boolean"));
-    rewrite plusnO; tcrush.
-  eapply Subs_typed_nocoerce.
+  rewrite /htrueTm/= -(iterate_S tskip 0).
+  apply (Subs_typed (T1 := hclose (▶ hpx (length Γ'') @; "Boolean")));
+    rewrite /= plusnO; tcrush.
+    eapply Subs_typed_nocoerce.
   - eapply TMuE_typed'; first eapply Var_typed'; by [rewrite lookup_app_r ?Nat.sub_diag|].
   - repeat lNext.
 Qed.
 
-Lemma falseTyp Γ Γ'' : Γ'' ++ boolImplT :: Γ u⊢ₜ falseTm.|[ren (+length Γ'')] : p0.|[ren (+length Γ'')] @; "Boolean".
+Lemma falseTyp Γ Γ'' : Γ'' ++ boolImplT :: Γ u⊢ₜ
+  hclose (hfalseTm (hx (length Γ''))) : hclose (hpx (length Γ'') @; "Boolean").
 Proof.
   have ?: length Γ'' < length (Γ'' ++ boolImplT :: Γ) by rewrite app_length /=; lia.
-  rewrite /falseTm /= -(iterate_S tskip 0).
-  apply (Subs_typed (T1 := ▶ pv (ids (length Γ'')) @; "Boolean"));
-    rewrite plusnO; tcrush.
+  rewrite /hfalseTm /= -(iterate_S tskip 0).
+  apply (Subs_typed (T1 := hclose (▶ hpx (length Γ'') @; "Boolean")));
+    rewrite /= plusnO; tcrush.
   eapply Subs_typed_nocoerce.
   - eapply TMuE_typed'; first eapply Var_typed'; by [rewrite lookup_app_r ?Nat.sub_diag|].
   -
@@ -40,83 +44,82 @@ Proof.
     repeat lNext.
 Qed.
 
-
-Definition nilV : vl := ν {@ (* self => *)
+Definition hnilV bool : hvl := ν: self, {@
   type "A" = ⊥;
-  val "isEmpty" = vabs (* d => *) (trueTm.|[ren (+2)]); (* for self and d *)
-  val "head" = vabs loopTm;
-  val "tail" = vabs loopTm
+  val "isEmpty" = λ: _, htrueTm bool;
+  val "head" = λ: _, pureS loopTm;
+  val "tail" = λ: _, pureS loopTm
 }.
 
 (*
   λ(x: {A})λ(hd: x.A)λ(tl: sci.List∧{A <: x.A}) let result = ν(self) {
     A = x.A; isEmpty = bool.false; head = hd; tail = tl } in result *)
-Definition consV : vl :=
-  vabs (* x => *) $ vabs' (* hd => *) $ vabs' (* tl => *) $ tv $ ν {@ (* self => *)
-    type "A" = p3 @; "T";
-    val "isEmpty" = vabs (* d => *) falseTm.|[ren (+5)];
-    val "head" = vabs (* d => *) (tv x3);
-    val "tail" = vabs (* d => *) (tv x2)
+Program Definition hconsV bool : hvl :=
+  λ: x, λ:: hd tl, htv $ ν: self, {@
+    type "A" = hpv x @; "T";
+    val "isEmpty" = λ: _, hfalseTm bool;
+    val "head" = λ: _, htv hd;
+    val "tail" = λ: _, htv tl
   }.
 
-Definition listTBodyGen L U := μ {@ (* self => *)
-  type "A" >: shift L <: shift U;
-  val "isEmpty" : ⊤ →: p2 @; "Boolean"; (* bool.Boolean *)
-  val "head" : ⊤ →: p0 @; "A"; (* self.A *)
-  val "tail" : ⊤ →: TAnd (p1 @; "List") (type "A" >: ⊥ <: p0 @; "A" )
+Definition hlistTBodyGen bool sci (L U : hty) : hty := μ: self, {@
+  type "A" >: L <: U;
+  val "isEmpty" : ⊤ →: hpv bool @; "Boolean";
+  val "head" : ⊤ →: hpv self @; "A";
+  val "tail" : ⊤ →: hTAnd (hpv sci @; "List") (type "A" >: ⊥ <: hpv self @; "A" )
 }.
 
-Definition listTBody := listTBodyGen ⊥ ⊤.
+Definition hlistTBody bool sci := hlistTBodyGen bool sci ⊥ ⊤.
 
-Definition listV : vl := ν {@ (* sci => *)
-  type "List" = listTBody; (* [shift] is for [sci] *)
-  val "nil" = shiftV nilV;
-  val "cons" = shiftV consV
+Definition hlistV bool : hvl := ν: self, {@
+  type "List" = hlistTBody bool self;
+  val "nil" = hnilV bool;
+  val "cons" = hconsV bool
 }.
 
-Definition nilT sci := TAnd (▶ sci @; "List") (typeEq "A" ⊥).
+Definition hnilT sci := hTAnd (▶ hpv sci @; "List") (typeEq "A" ⊥).
 
 (** ∀(x: {A})∀(hd: x.A)∀(tl: sci.List∧{A <: x.A})sci.List∧{A <: x.A} *)
-Definition consT sci : ty :=
-  TAll (tparam "T")
-    (p0 @; "T" →:
-    (TAnd (shift sci @; "List") (type "A" >: ⊥ <: p0 @; "T")) →:
-    TAnd (shift sci @; "List") (type "A" >: ⊥ <: p0 @; "T")).
+Definition hconsT sci : hty :=
+  ∀: x : (tparam "T"),
+    hpv x @; "T" →:
+    (hTAnd (hpv sci @; "List") (type "A" >: ⊥ <: hpv x @; "T")) →:
+    hTAnd (hpv sci @; "List") (type "A" >: ⊥ <: hpv x @; "T").
 
-Definition listT : ty := μ {@ (* sci => *)
-  type "List" >: ⊥ <: listTBody; (* [shift] is for [sci] *)
-  val "nil" : nilT p0;
-  val "cons" : consT p0
+Definition hlistT bool : hty := μ: sci, {@
+  type "List" >: ⊥ <: hlistTBody bool sci;
+  val "nil" : hnilT sci;
+  val "cons" : hconsT sci
 }.
 
-Definition consTResConcr U : ty := listTBodyGen U U.
-Definition consTConcr sci : ty :=
-  TAll (tparam "T")
-    (p0 @; "T" →:
-      TAnd (shift sci @; "List") (type "A" >: ⊥ <: p0 @; "T") →:
-      (* This renaming is needed because I'm inserting a local variable that isn't expected by
-      [consTResConcr] *and I'm using it in the argument*. I could also just clone *)
-      (consTResConcr (p2 @; "T")).|[ids 1 .: ids 2 .: ids 0 .: ids]).
+Definition hconsTResConcr bool sci U := hlistTBodyGen bool sci U U.
 
-      (* (consTResConcr (p2 @; "T")).|[∞ [ids 1 ; ids 2 ; ids 0]]). *)
-Definition listTConcrBody : ty := {@ (* sci => *)
-  typeEq "List" $ listTBody; (* [shift] is for [sci] *)
-  val "nil" : nilT p0;
-  val "cons" : consTConcr p0
+Definition hconsTConcr bool sci : hterm ty :=
+  ∀: x: tparam "T",
+    hpv x @; "T" →:
+      hTAnd (hpv sci @; "List") (type "A" >: ⊥ <: hpv x @; "T") →:
+      (hconsTResConcr bool sci (hpv x @; "T")).
+
+Definition hlistTConcrBody bool sci : hty := {@
+  typeEq "List" $ hlistTBody bool sci;
+  val "nil" : hnilT sci;
+  val "cons" : hconsTConcr bool sci
 }.
 
-Definition listTConcr : ty := μ listTConcrBody.
+Definition hlistTConcr bool : hty := μ: sci, hlistTConcrBody bool sci.
 
-Definition nilTConcr : ty := listTBodyGen ⊥ ⊥.
+Definition hnilTConcr bool sci : hty := hlistTBodyGen bool sci ⊥ ⊥.
 
-Example nilTyp Γ : (▶ listTConcrBody)%ty :: boolImplT :: Γ u⊢ₜ shift (tv nilV) : nilT p0.
+Example nilTyp Γ : hclose (▶ hlistTConcrBody hx1 hx0) :: boolImplT :: Γ u⊢ₜ
+  hclose (htv (hnilV hx1)) : hclose (hnilT hx0).
 Proof.
-  apply (Subs_typed_nocoerce nilTConcr).
+  apply (Subs_typed_nocoerce $ hclose $ hnilTConcr hx1 hx0).
   - evar (T : ty).
-    have := trueTyp Γ [⊤; T; ▶ listTConcrBody]%ty.
-    have := loopTyp (⊤ :: T :: ▶ listTConcrBody :: boolImplT :: Γ)%ty.
+    set L :=  hclose (▶ hlistTConcrBody hx1 hx0).
+    have := trueTyp Γ [hclose ⊤; T; L].
+    have := loopTyp (hclose ⊤ :: T :: L :: boolImplT :: Γ).
     rewrite {}/T/= => Ht Hl.
-    tcrush; apply (Subs_typed_nocoerce ⊥); tcrush.
+    tcrush; apply (Subs_typed_nocoerce (hclose ⊥)); cbn; tcrush.
   - tcrush; last (apply Bind1; tcrush).
     ettrans; first eapply TAddLater_stp; stcrush.
     asideLaters.
@@ -125,16 +128,17 @@ Proof.
     lThis. lThis.
 Qed.
 
-Example consTyp Γ :
-  (▶ listTConcrBody)%ty :: boolImplT :: Γ u⊢ₜ shift (tv consV) : consTConcr p0.
+Example consTyp Γ : hclose (▶ hlistTConcrBody hx1 hx0) :: boolImplT :: Γ u⊢ₜ
+  hclose (htv (hconsV hx1)) : hclose (hconsTConcr hx1 hx0).
 Proof.
   epose proof falseTyp Γ [_; _; _; _; _; _] as Ht; cbn in Ht.
-  tcrush; clear Ht; first by varsub; eapply (LSel_stp' _ (p4 @; "T")); tcrush; varsub; lThis.
+  tcrush; clear Ht; first by varsub; eapply (LSel_stp' _ (hclose (hp4 @; "T"))); tcrush; varsub; lThis.
   hideCtx. varsub. tcrush. lNext.
   eapply LSel_stp'; tcrush. varsub. lThis.
 Qed.
 
-Lemma consTSub Γ : listTConcrBody :: boolImplT :: Γ u⊢ₜ consTConcr p0, 0 <: consT p0, 0.
+Lemma consTSub Γ : hclose (hlistTConcrBody hx1 hx0) :: boolImplT :: Γ u⊢ₜ
+  hclose (hconsTConcr hx1 hx0), 0 <: hclose (hconsT hx0), 0.
 Proof.
   tcrush; rewrite !iterate_S !iterate_0; hideCtx.
   eapply LSel_stp'; tcrush. varsub. tcrush. lThis.
@@ -142,19 +146,19 @@ Proof.
   apply Bind1; stcrush. by lThis.
 Qed.
 
-Example listTypConcr Γ : boolImplT :: Γ u⊢ₜ tv listV : listTConcr.
+Example listTypConcr Γ : boolImplT :: Γ u⊢ₜ hclose (htv (hlistV hx0)) : hclose (hlistTConcr hx0).
 Proof.
   have Hn := nilTyp Γ.
   (* Without the call to [dvl_typed], Coq would (smartly) default to [dvabs_typed] *)
-  have := consTyp Γ => /(dvl_typed "cons") Hc.
+  have := consTyp Γ => /(dvl_typed "cons") Hc /=.
   tcrush.
 Qed.
 
-Example listTyp Γ : boolImplT :: Γ u⊢ₜ tv listV : listT.
+Example listTyp Γ : boolImplT :: Γ u⊢ₜ hclose (htv (hlistV hx0)) : hclose (hlistT hx0).
 Proof.
   have Hv := listTypConcr Γ.
   have Hsub := consTSub Γ.
-  apply (Subs_typed_nocoerce listTConcr); tcrush.
+  eapply Subs_typed_nocoerce; first exact Hv; tcrush.
   lThis.
   lNext.
   do 2 lNext; lThis.
@@ -171,11 +175,17 @@ Example clListTyp Γ : Γ u⊢ₜ clListV : listT.
   Fail change (shift listT) with (listT).
   Fail apply listTyp.
 Abort. *)
+Definition hvabs' x := htv (hvabs x).
+Definition hlett t u := htapp (hvabs' u) t.
+Arguments hvabs' /.
+Arguments hlett /.
+(* Notation "hlett: x := t in u" := (htapp (λ: x, u) t) (at level 200). *)
 
-Definition clListV' body := lett (tv boolImpl) $ lett (tv listV) body.
-Example clListTyp' Γ T body
-  (Ht : shift listT :: boolImplT :: Γ u⊢ₜ body : shift (shift T)) :
-  Γ u⊢ₜ clListV' body : T.
+(* Try1, working well? *)
+Definition clListV' body := hlett (htv (pureS boolImpl)) (λ bool, hlett (htv (hlistV bool)) (λ list, pureS body)).
+Example clListTyp' Γ (T : ty) body
+  (Ht : shift (hclose (hlistT hx0)) :: boolImplT :: Γ u⊢ₜ body : shift (shift T)) :
+  Γ u⊢ₜ hclose (clListV' body) : T.
 Proof.
   eapply Let_typed; first apply boolImplTyp.
   eapply Let_typed; first apply listTyp.
@@ -183,7 +193,33 @@ Proof.
 Qed.
 
 Example clListTypNat Γ :
-  Γ u⊢ₜ clListV' (tv (vnat 1)) : 𝐍.
+  Γ u⊢ₜ hclose (clListV' (hclose (htv (hvnat 1)))) : hclose 𝐍.
 Proof. apply clListTyp'. tcrush. Qed.
+
+
+
+(* Try2. Try taking a HOAS body. Works less well. *)
+
+(* Argh. Variable by de Bruijn level. Not good. *)
+Definition hxm i : hvl := λ j, var_vl (j - i).
+Definition hxm' i : hvl := ren (λ j, j - i).
+Goal hxm = hxm'. done. Qed.
+
+Definition clListV'2 body := hlett (htv (pureS boolImpl)) (λ bool, hlett (htv (hlistV bool)) (λ list, body bool list)).
+(* Definition clListV' body := hlett: bool := (htv (pureS boolImpl)), hlett (htv (hlistV bool)) body. *)
+Example clListTyp'2 Γ (T : ty) body
+  (* (Ht : hclose (hlistT hx1) :: boolImplT :: Γ u⊢ₜ hclose (body hx1 hx0) : shift (shift T)) : *)
+  (Ht : shift (hclose (hlistT hx0)) :: boolImplT :: Γ u⊢ₜ (body (hxm 1) (hxm 2)) 2 : shift (shift T)) :
+  (* (Ht : shift (hclose (hlistT hx0)) :: boolImplT :: Γ u⊢ₜ hclose (body (hx (-1)) (hx (-2)) 2 : shift (shift T)) : *)
+  Γ u⊢ₜ hclose (clListV'2 body) : T.
+Proof.
+  eapply Let_typed; first apply boolImplTyp.
+  eapply Let_typed; first apply listTyp.
+  all: tcrush.
+Qed.
+
+Example clListTypNat2 Γ :
+  Γ u⊢ₜ hclose (clListV'2 (λ _ _, htv (hvnat 1))) : hclose 𝐍.
+Proof. apply clListTyp'2. tcrush. Qed.
 
 (* Try recursive linking? *)
